{
 "cells": [
  {
   "cell_type": "markdown",
   "metadata": {},
   "source": [
    "# MATH97018, MATH97096: Problem Sheet 2 Solutions"
   ]
  },
  {
   "cell_type": "markdown",
   "metadata": {},
   "source": [
    "## 1."
   ]
  },
  {
   "cell_type": "markdown",
   "metadata": {},
   "source": [
    "We will consider the Michaelis-Menten system\n",
    "\n",
    "\\begin{align*}\n",
    "\\epsilon\\frac{dv}{d\\tau} &= u - (u + K)v,\\\\\n",
    "\\frac{du}{d\\tau} &= -u + (u + K - \\lambda)v \n",
    "\\end{align*}\n",
    "\n",
    "\\begin{enumerate}\n",
    "\n",
    "\\item We first rescale time such that $\\tau = \\epsilon T$, and write $U(T) = u(\\tau)$ and $V(T) = v(\\tau)$. Then the system becomes\n",
    "\n",
    "\\begin{align*}\n",
    "\\frac{dV}{dT} &= U - (U + K)V,\\\\\n",
    "\\frac{dU}{dT} &= \\epsilon[-U + (U + K - \\lambda)V],\n",
    "\\end{align*}\n",
    "and we have initial conditions $U(0) = 1$, $V(0) = 0$.\n",
    "\n",
    "\\item Expanding the solution as a power series in $\\epsilon$ gives\n",
    "\n",
    "\\begin{align*}\n",
    "V &= V_{0} + \\epsilon V_{1} + O(\\epsilon^2),\\\\\n",
    "U &= U_{0} + \\epsilon U_{1} + O(\\epsilon^2).\\\\\n",
    "\\end{align*}\n",
    "\n",
    "Substituting this series into the equations found in (i), we have \n",
    "\n",
    "\\begin{align*}\n",
    "\\frac{dU_{0}}{dT} &= 0, \\\\\n",
    "\\frac{dV_{0}}{dT} &= U_{0} - (U_{0} + K)V_{0},\n",
    "\\end{align*}\n",
    "\n",
    "at leading order.  The first equation with the initial condition $U(0) = 1$ gives $U_{0}(T) = 1$.  Substituting this into the differential equation for $V_{0}$ gives\n",
    "\n",
    "\\begin{align*}\n",
    "\\frac{dV_{0}}{dT} = 1 - (1 + K)V_{0}\\\\\n",
    "\\end{align*}\n",
    "\n",
    "which, with the initial condition, $V(0) = 0$ has solution\n",
    "\n",
    "\\begin{align*}\n",
    "V_{0}(T) = \\frac{1}{1+K}\\left( 1 - \\text{e}^{-(1+K)T}\\right)\n",
    "\\end{align*}\n",
    "\n",
    "\n",
    "\\item Recall the solution obtained using the quasi-steady hypothesis: \n",
    "\n",
    "\\begin{align*}\n",
    "u(\\tau) + K\\log{u(\\tau)} &= 1-\\lambda\\tau \\\\\n",
    "v(\\tau) = u(\\tau)/(u(\\tau)+K).\\\\\n",
    "\\end{align*}\n",
    "\n",
    "Taking the limit as $\\tau \\rightarrow 0$ gives\n",
    "\n",
    "\\begin{align*}\n",
    "\\lim_{\\tau\\rightarrow 0 }[u(\\tau),v(\\tau)] = \\bigg[1, \\frac{1}{1+K}\\bigg].\n",
    "\\end{align*}\n",
    "\n",
    "Taking the limit as $T \\rightarrow \\infty$ for $U_0(T)$ and $V_0(T)$, we have \n",
    "\\begin{align*}\n",
    "\\lim_{T \\rightarrow \\infty }[U_0(T),V_0(T)] = \\bigg[1, \\frac{1}{1+K}\\bigg],\n",
    "\\end{align*}\n",
    "which matches.\n",
    "\n",
    "\\item Using this limit, we then have\n",
    "\\begin{align*}\n",
    "u(\\tau) + U_0({\\tau/\\epsilon}) - \\lim_{T\\rightarrow \\infty}U_0 &= 1-\\lambda\\tau-K\\log u\n",
    "\\end{align*}\n",
    "and\n",
    "\\begin{align*}\n",
    "v(\\tau) + V_0({\\tau/\\epsilon}) - \\lim_{T\\rightarrow \\infty}V_0 &= \\frac{u}{u+K} - \\frac{1}{1+K}\\text{e}^{-(1+K)\\tau/\\epsilon}\n",
    "\\end{align*}\n",
    "\n",
    "\\item Experimenting with the code, we can confirm that the analytical solution approaches the numerical solution as $\\epsilon \\rightarrow 0$.  The discrepancy appears primarily in $u(\\tau)$ with the numerical solution exhibiting an $O(\\epsilon)$ intial decay that is not present in the analytical solution.\n",
    "\\end{enumerate}"
   ]
  },
  {
   "cell_type": "markdown",
   "metadata": {},
   "source": [
    "## 2.\n",
    "\\begin{enumerate} \n",
    "\\item The system of ODE's describing this reaction are \n",
    "\n",
    "\\begin{align*}\n",
    "\\frac{de}{dt} &= 2c-es\\ \\\\\n",
    "\\frac{dc}{dt} &= es-2c \\\\\n",
    "\\frac{dp}{dt} &= c \\\\\n",
    "\\frac{ds}{dt} &= c-es.\n",
    "\\end{align*}\n",
    "\n",
    "Then $$ \\frac{de}{dt}+\\frac{dc}{dt} = 0 \\iff e+c = C \\text{ where $C$ is constant }  $$\n",
    "\n",
    "By initial conditions we have that $e+c = e_0 \\Rightarrow e = e_0 - c$. Furthermore we note that $p$ can be computed once $c$ is known. Thus, we need only consider the ODEs for $s$ and $c$.  Using $e = e_0 - c$, we have\n",
    "\n",
    "\\begin{align*}\n",
    "\\frac{ds}{dt} &= c-(e_0-c)s \\\\\n",
    "\\frac{dc}{dt} &= (e_0-c)s-2c \n",
    "\\end{align*}\n",
    "\n",
    "Substituting $c(t)=e_0v(t)$ into the equations above gives  \n",
    "\n",
    "\\begin{align*}\n",
    "\\frac{ds}{dt} &= e_0(v-(1-v)s) \\\\\n",
    "\\frac{dv}{dt} &= (1-v)s-2v\n",
    "\\end{align*}\n",
    "\n",
    "\\item The Michaelis-Menten quasi-steady approximation states that since only a small amount of enzyme is required, $e_0 << 1$, we have that the substrate concentration remains constant while the complex concentration reaches its fixed point (steady state) value.  Thus, we consider\n",
    "\\begin{align*}\n",
    "\\frac{ds}{dt} &= e_0(v-(1-v)s) \\\\\n",
    "0 &= (1-v)s-2v\n",
    "\\end{align*}\n",
    "Solving the algebraic equation for $v$ gives $v = s/(s + 2)$.  After substituting this expression for $v$ into the differential equation for $s$ and rearranging, we obtain\n",
    "\n",
    "\\begin{align*}\n",
    "\\frac{ds}{dt} = -e_0\\frac{s}{s+2}.\n",
    "\\end{align*}\n",
    "\n",
    "The solution to this equation that satisfies $s(0) = s_0$ is\n",
    "\n",
    "\\begin{align*}\n",
    "s+ 2\\log(s) = s_0 + 2\\log(s_0) - e_0 t. \n",
    "\\end{align*}\n",
    "\n",
    "\\item Since $ds/dt < 0$, $s$ will decrease from $s_0$ and $s\\rightarrow 0$ as $t\\rightarrow \\infty$.  At large times then, the term $2\\log s$ on the left-hand side will balance the right-hand side.  Thus, we take $2 \\log s = s_0 + 2 \\log s_0 - e_0 t$, or $s = s_0 \\exp\\big[ \\frac{1}{2}(s_0 âˆ’ e_0t)\\big]$.\n",
    "\n",
    "\\item Initially $s\\approx s_0$ while $v$ evolves. Thus, \n",
    "\n",
    "\\begin{align*}\n",
    "\\frac{dv}{dt} &= s_0 - (s_0+2)v\n",
    "\\end{align*}\n",
    "\n",
    "with initial condition $v(0) = 0$. This has solution \n",
    "\n",
    "\\begin{align*}\n",
    "v = \\frac{s_0}{s_0+2} (1 - \\exp[-(s_0+2)t])\n",
    "\\end{align*}\n",
    "\n",
    "and we see that $v \\rightarrow s_0/(s_0+2)$ as $t \\rightarrow \\infty$.\n",
    "\\end{enumerate}"
   ]
  },
  {
   "cell_type": "markdown",
   "metadata": {},
   "source": [
    "## 3."
   ]
  },
  {
   "cell_type": "markdown",
   "metadata": {},
   "source": [
    "\\begin{enumerate} \n",
    "\\item There are two time scales here, $r^{-1}_1$ and $r^{-1}_2$.  Given the final non-dimensional equations, it is clear that the former has been used to non-dimensionalise time and take $T = t/r_1$. Then, we scale $N_1$ by $K_1$ and $N_2$ by $K_2$, introducing $N_1 = K_1u_1$ and $N_2 = K_2u_2$. Using the new variables, we obtain\n",
    "\n",
    "\\begin{align*}\n",
    "r_1K_1\\frac{du_1}{dt} &= r_1K_1u_1(1-\\frac{K_1u_1}{K_1}+b_{12}\\frac{K_2u_2}{K_1})\\\\\n",
    "r_1K_2\\frac{du_2}{dt} &= r_2K_2u_2(1-\\frac{K_2u_2}{K_2}+b_{21}\\frac{K_1u_1}{K_2})\\,,\n",
    "\\end{align*}\n",
    "\n",
    "which simplifies to\n",
    "\n",
    "\\begin{align}\n",
    "\\frac{du_1}{dt} &= u_1(1 - u_1 + \\alpha_{12}u_2 ) \\label{eq:star}\\\\\n",
    "\\frac{du_2}{dt} &= \\rho u_2(1 - u_2 + \\alpha_{21}u_1 ) \\label{eq:starstar} \n",
    "\\end{align}\n",
    "\n",
    "where $\\rho = r_2/r_1$ and $\\alpha_{12} = b_{12} K_2/K_1$ and $\\alpha_{21} = b_{21}K_1/K_2$.\n",
    "\n",
    "\\item We seek steady states by letting $f(u_1,u_2) = 0$ and $g(u_1,u_2) = 0$.  We have $f(u_1,u_2) = 0$ if $u_1^* = 0$, then $g = 0$ when $u_2^* = 0$ or $u^*_2 = 1$. For $u_2^* = 0$, we may also have that $f = 0$ when $u_1^* = 1$. Hence we have the three steady states $(0,0), (1,0), (0,1)$. Additionally, $f = 0$ when $u_2^* = \\frac{u_1 -1}{\\alpha_{12}}$. Substituting this into $g = 0$ we find $u_1 = \\frac{(1+\\alpha_{12})}{1-\\alpha_{21}\\alpha_{12}}$ and $u_2=\\frac{(1+\\alpha_{12})}{1-\\alpha_{12}\\alpha_{21}}$. So we also have steady state \n",
    "\n",
    "\\begin{align*}\n",
    "(u^*, v^*) = \\frac{1}{1-\\alpha_{12}\\alpha_{21}}(1+\\alpha_{12},1+\\alpha_{21}).\n",
    "\\end{align*}\n",
    "\n",
    "The Jacobian of the system is \n",
    "\n",
    "\\begin{align*}\n",
    "J = \n",
    "\\begin{pmatrix}\n",
    "1-2u_1^* + \\alpha_{12}u_2^* & \\alpha_{12}u_1^* \\\\\n",
    "\\rho \\alpha_{21}u_2^* & \\rho(1-2u_2^*+\\alpha_{21}u_1^*) \n",
    "\\end{pmatrix}\n",
    "\\end{align*}\n",
    "\n",
    "At $(u_1^*,u_2^*) = (0,0)$\n",
    "\n",
    "\\begin{align*}\n",
    "J = \n",
    "\\begin{pmatrix}\n",
    "1 & 0 \\\\\n",
    "0 & \\rho\n",
    "\\end{pmatrix}\n",
    "\\end{align*}\n",
    "\n",
    "with eigenvalues $\\lambda = 1, \\rho$. Therefore $(0,0)$ is an unstable node. \n",
    "\n",
    "At $(u_1^*,u_2^*) = (1,0)$\n",
    "\n",
    "\\begin{align*}\n",
    "J = \n",
    "\\begin{pmatrix}\n",
    "-1 & \\alpha_{12} \\\\\n",
    "0 & \\rho(1+\\alpha_{21})\n",
    "\\end{pmatrix}\n",
    "\\end{align*}\n",
    "\n",
    "with eigenvalues $\\lambda = -1, \\rho(1+\\alpha_{21})$. Therefore $(1,0)$ is a saddle and always unstable. \n",
    "\n",
    "At $(u_1^*,u_2^*) = (0,1)$\n",
    "\n",
    "\\begin{align*}\n",
    "J = \n",
    "\\begin{pmatrix}\n",
    "1+\\alpha_{12} & 0 \\\\\n",
    "\\rho \\alpha_{21} & -\\rho\n",
    "\\end{pmatrix}\n",
    "\\end{align*}\n",
    "\n",
    "with eigenvalues $\\lambda = -\\rho, 1+\\alpha_{12}$. Therefore $(0,1)$ is a saddle and always unstable.\n",
    "\n",
    "\\item For fixed point $(u_1^*,u_2^*) = \\frac{1}{1-\\alpha_{12}\\alpha_{21}}(1+\\alpha_{12},1+\\alpha_{21})$, if $\\alpha_{12}\\alpha_{21} > 1$, then $u^*_1 < 0$ and $u^*_2 < 0$ and are, therefore, inadmissible.  As a result, any initial condition in the positive quadrant will result in a trajectory that moves to the region where $f > 0$ and $g > 0$ and the populations will grown without bound.\n",
    "\n",
    "If $\\alpha_{12}\\alpha_{21} < 1$, then $u^*_1 > 0$ and $u^*_2 > 0$ and we will have an additional fixed point with Jacobian\n",
    "\n",
    "\\begin{align*}\n",
    "J = \n",
    "\\begin{pmatrix}\n",
    "-u_1^* & \\alpha_{12}u_1^* \\\\\n",
    "\\rho\\alpha_{21}u_2^* & -\\rho u_2^*\n",
    "\\end{pmatrix}\n",
    "\\end{align*}\n",
    "\n",
    "which has $\\text{trace}(J) = -\\rho u^*_1 - u^*_2$ and $\\text{det}(J) = \\rho u_1^* u_2^* (1-\\alpha_{12}\\alpha_{21})$.  Since the trace is positive and the determinant is negative the fixed point is either a stable node or stable spiral.\n",
    "\\end{enumerate} "
   ]
  },
  {
   "cell_type": "markdown",
   "metadata": {},
   "source": [
    "## 4."
   ]
  },
  {
   "cell_type": "markdown",
   "metadata": {},
   "source": [
    "\\begin{enumerate}\n",
    "\n",
    "\\item For large $N$, $\\gamma f(N) \\sim \\gamma$ and so the per-predator rate of predation saturates. For small $N$,\n",
    "$\\gamma f(N) \\sim \\gamma N/D$ and so the per-predator rate of predation increases linearly.\n",
    "\n",
    "\\item Using the scalings provided in the question, we have \n",
    "\n",
    "\\begin{align*}\n",
    "\\rho K \\frac{du}{d\\tau} &= \\rho uK\\left(1-\\frac{Ku}{K}\\right) - \\gamma v\\frac{\\rho K}{\\gamma}\\bigg(\\frac{Ku}{Ku+D}\\bigg)\\\\\n",
    "\\frac{\\rho^2 K}{\\gamma}\\frac{dv}{d\\tau} &= \\frac{\\rho K}{\\gamma}v\\bigg( \\frac{\\sigma u}{u+D/K} - \\eta \\bigg)\n",
    "\\end{align*}\n",
    "\n",
    "Hence,\n",
    "\n",
    "\\begin{align*}\n",
    "\\frac{du}{d\\tau} &= u(u-1) -v\\bigg( \\frac{u}{u+\\delta} \\bigg) = f_1(u,v) \\\\\n",
    "\\frac{dv}{d\\tau} &= v\\bigg( \\lambda \\frac{u}{u+D/K} -\\mu \\bigg) = f_2(u,v)\n",
    "\\end{align*}\n",
    "\n",
    "where $\\delta = D/K, \\lambda = \\sigma/\\rho, \\mu = \\eta/\\rho$.\n",
    "\n",
    "\\item If $v = 0$, then we have automatically that $f_2(u,0) = 0$ and that $f_1(u,0) = u(u-1)$.  Thus, $(0,0)$ and $(1,0)$ are fixed points. \n",
    "\n",
    "We now look for the third steady state. We note that $f_2(u,v) = 0$ when $v=0$ or $(\\frac{\\lambda u }{u+\\delta} - \\mu) = 0$.  The first has already been considered. The second is satisfied for $u^* = \\frac{\\delta \\mu}{\\lambda - \\mu }$. We now consider $f_1(u^*,v) = 0$ to find $v^*$. First we note \n",
    "\n",
    "\\begin{align*}\n",
    "f_1(u,v)= u(u-1) -v \\bigg( \\frac{u}{u+\\delta} \\bigg) \\\\\n",
    "= \\frac{u}{u+\\delta} [(1-u)(u+\\delta)-v].\n",
    "\\end{align*}\n",
    "\n",
    "So $v^*$ is such that the term inside the square brackets is zero at $u = u^*$, or\n",
    "\n",
    "\\begin{align*}\n",
    "v^* = \\bigg[ (1 - \\frac{\\delta \\mu }{\\lambda -\\mu})(\\frac{\\delta \\mu}{\\lambda-\\mu} +\\delta ) \\bigg]\\\\\n",
    "= \\frac{1}{(\\lambda-\\mu)^2}(\\lambda - \\mu - \\delta \\mu) (\\delta \\mu + \\delta (1-\\mu)) \\\\\n",
    "\\frac{\\delta\\lambda}{(\\lambda - \\mu)^2} (\\lambda - \\mu(1+\\delta))\n",
    "\\end{align*}\n",
    "\n",
    "which is positive when $\\lambda> \\mu(1+\\delta)$.\n",
    "\n",
    "\\item The Jacobian is \n",
    "\n",
    "\\begin{align*}\n",
    "J = \n",
    "\\begin{pmatrix}\n",
    "1-2u-\\delta\\frac{v}{(u+\\delta)^2} & -\\frac{u}{u+\\delta} \\\\\n",
    "\\delta\\lambda\\frac{v}{(u+\\delta)^2} & \\frac{\\lambda u}{u+\\delta}-\\mu\n",
    "\\end{pmatrix}\n",
    "\\end{align*}\n",
    "\n",
    "For (0,0) \n",
    "\n",
    "\\begin{align*}\n",
    "J = \\begin{pmatrix} 1 & 0 \\\\ 0 & -\\mu \\end{pmatrix},\n",
    "\\end{align*}\n",
    "\n",
    "which has eigenvalues $\\lambda_{1,2} = 1,-\\mu$ and is therefore a saddle and so unstable. \n",
    "\n",
    "For fixed point (1,0), we have\n",
    "\n",
    "\\begin{align*}\n",
    "J = \\begin{pmatrix} -1 & \\frac{-1}{1+\\delta} \\\\ 0 & \\frac{\\lambda}{1+\\delta}-\\mu \\end{pmatrix}.\n",
    "\\end{align*}\n",
    "\n",
    "This has eigenvalues $\\lambda_{1,2} = -1, \\lambda/(1+\\delta)-\\mu$.  If $\\lambda > \\mu(1 + \\delta)$, then $\\lambda_2$ is positive and we have a saddle.\n",
    "\n",
    "\n",
    "\\item Recalling that $v^* = (1-u^*)(u^* + \\delta)$, we then have $\\frac{\\delta v^*}{(u^* + \\delta)^2} = \\delta \\frac{(1-u^*)}{(u^* + \\delta)}$. Also we note that $\\frac{\\lambda u^*}{u^* + \\delta} = \\mu$. Using these identities we find the Jacobian at $(u^*, v^*)$ to be \n",
    "\n",
    "\\begin{align*}\n",
    "J = \\begin{pmatrix} 1 - 2u^* - \\delta \\frac{1-u^*}{u^* + \\delta} & -\\frac{u^*}{u^* + \\delta} \\\\ \\delta \\lambda \\frac{1-u^*}{u^* + \\delta} & 0 \\end{pmatrix}\n",
    "\\end{align*}\n",
    "\n",
    "We note further that we must have that $u^* \\leq 1$ so that $v^* \\geq 0$. The determinant is then $\\delta \\mu (1-u^*)/(u+\\delta) >0$. The trace is $1-2u^* -\\delta (1-u^*)/(u^*+\\delta) = (u^*/(u^* + \\delta))(1-2u^*-\\delta)$. Its sign is determined by the sign of the term inside the bracket. We have:\n",
    "\n",
    "$$\n",
    "(1-2u^* -\\delta) = 1-2\\frac{\\mu \\delta}{\\lambda - \\mu} -\\delta\\\\\n",
    "= \\frac{\\lambda-\\mu -2\\mu\\delta -\\delta (\\lambda-\\mu)}{\\lambda-\\mu}\\\\\n",
    "= \\frac{\\lambda(1-\\delta)-\\mu(1+\\delta)}{\\lambda-\\mu}\n",
    "$$\n",
    "\n",
    "The denominator is always positive by previous assumptions $(\\lambda > \\mu(1+\\delta))$. For stability we need the trace to be negative and hence we must have that $\\lambda(1-\\delta) - \\mu (1+\\delta)<0$ and the result follows. \n",
    "\\end{enumerate}"
   ]
  },
  {
   "cell_type": "markdown",
   "metadata": {},
   "source": [
    "## 5.\n",
    "\n",
    "The criss-cross infection model is given by\n",
    "\n",
    "\\begin{align*}\n",
    "\\frac{dS}{dt} &= -r SI', \\\\\n",
    "\\frac{dI}{dt} &= rSI'-aI, \\\\\n",
    "\\frac{dR}{dt} &= aI, \\\\\n",
    "\\frac{dS'}{dt} &= -r'S'I',\\\\\n",
    "\\frac{dI'}{dt} &= r'S'I - a'I',\\\\\n",
    "\\frac{dR'}{dt} &= a'I'.\n",
    "\\end{align*}\n",
    "\n",
    "\\begin{enumerate}\n",
    "\\item For the male population, we have $N = S + I + R$.  Thus,\n",
    "\n",
    "\\begin{align*}\n",
    "\\frac{dN}{dt} &= \\frac{dS}{dt} + \\frac{dI}{dt} + \\frac{dR}{dt}\\\\\n",
    "&= -r SI' + rSI'-aI +aI \\\\\n",
    "&= 0.\n",
    "\\end{align*}\n",
    "\n",
    "Similarly, for the female population, $N' = S' + I' + R'$, we have\n",
    "\n",
    "\\begin{align*}\n",
    "\\frac{dN'}{dt} &= \\frac{dS'}{dt} + \\frac{dI'}{dt} + \\frac{dR'}{dt}\\\\\n",
    "&= -r' S'I + r'S'I-a'I' +a'I' \\\\\n",
    "&= 0.\n",
    "\\end{align*}\n",
    "\n",
    "To show that $S(t) = S_0 \\exp [-r R' / a']$, we begin by using the equation\n",
    "\n",
    "\\begin{align*}\n",
    "\\frac{dR'}{dt} = a'I\n",
    "\\end{align*}\n",
    "\n",
    "to express the equation for the male susceptible population,\n",
    "\n",
    "\\begin{align*}\n",
    "\\frac{dS}{dt} &= -rSI', \\\\\n",
    "\\end{align*}\n",
    "\n",
    "as\n",
    "\n",
    "\\begin{align*}\n",
    "\\frac{dS}{dt} = \\frac{-rS}{a'}\\frac{dR'}{dt}. \\\\\n",
    "\\end{align*}\n",
    "\n",
    "Upon separating variables, we have \n",
    "\n",
    "\\begin{align*}\n",
    "\\frac{1}{S}\\frac{dS}{dt} = \\frac{-r}{a'}\\frac{dR'}{dt}.\n",
    "\\end{align*}\n",
    "\n",
    "Integrating both sides in time,\n",
    "\n",
    "\\begin{align*}\n",
    "\\int_{S(0)}^{S(t)} \\frac{1}{S} dS = \\int_{R'(0)}^{R'(t)} \\frac{-r}{a'} dR', \\\\\n",
    "\\end{align*}\n",
    "we obtain\n",
    "\\begin{align*}\n",
    "S(t) = S_0 \\exp(-rR'/a')\n",
    "\\end{align*}\n",
    "\n",
    "By similar arguments, we have that\n",
    "\n",
    "\\begin{align*}\n",
    "S'(t) = S_0' \\exp(-r'R/a)\n",
    "\\end{align*}\n",
    "\n",
    "\\item Since,\n",
    "\n",
    "\\begin{align*}\n",
    "N' = S'+I'+R',\n",
    "\\end{align*}\n",
    "\n",
    "we have \n",
    "\n",
    "\\begin{align*}\n",
    "N'\\geq R'(t) \\geq 0.\n",
    "\\end{align*}\n",
    "\n",
    "Also, since\n",
    "\n",
    "\\begin{align*}\n",
    "R'(t) = \\int_{0}^t I'(\\tau) d\\tau\n",
    "\\end{align*}\n",
    "\n",
    "and $I'(t)$ is strictly positive, $R'(t)$ is monotonically increasing. \n",
    "\n",
    "Thus, $R'$ attains its largest value as $t\\rightarrow \\infty$.\n",
    "\n",
    "Therefore, since $S'$ monotonically decreases with $R'$, \n",
    "\n",
    "\\begin{align*}\n",
    "S(\\infty) \\geq S_0 \\exp(-rN'/a') > 0\n",
    "\\end{align*}\n",
    "\n",
    "Similar arguments give\n",
    "\n",
    "\\begin{align*}\n",
    "S'(\\infty) \\geq S'_0 \\exp(-r'N/a) >0\n",
    "\\end{align*}\n",
    "\n",
    "Since, \n",
    "\n",
    "\\begin{align*}\n",
    "N\\geq R(t) = \\int_0^t I(\\tau) d\\tau\n",
    "\\end{align*}\n",
    "\n",
    "and $I(t)$ is positive, the integral must converge.  Thus, $I(t) \\rightarrow 0$ as $t \\rightarrow \\infty$.\n",
    "\n",
    "By similar arguments, \n",
    "\n",
    "\\begin{align*}\n",
    "I'(t) \\rightarrow 0 \\text{ as } t \\rightarrow \\infty \n",
    "\\end{align*}\n",
    "\n",
    "\\item An epidemic occurs if $\\frac{dI}{dt}>0$ or $\\frac{dI'}{dt}> 0$ at $t = 0$.  Thus, we consider\n",
    "\n",
    "\\begin{align*}\n",
    "\\frac{dI}{dt}(0) &= rS_0I_0' - aI_0 >0 \\\\\n",
    "\\frac{dI'}{dt}(0) &= r'S_0'I_0 - a'I_0'>0 \n",
    "\\end{align*}\n",
    "\n",
    "which give that\n",
    "\n",
    "\\begin{align*}\n",
    "\\frac{S_0I_0'}{I_0} &> \\frac{a}{r} \\\\\n",
    "\\frac{S'_0I_0}{I'_0} &>\\frac{a'}{r'}\n",
    "\\end{align*}\n",
    "for an epidemic to occur.  \n",
    "\\end{enumerate}"
   ]
  }
 ],
 "metadata": {
  "kernelspec": {
   "display_name": "Python 3",
   "language": "python",
   "name": "python3"
  },
  "language_info": {
   "codemirror_mode": {
    "name": "ipython",
    "version": 3
   },
   "file_extension": ".py",
   "mimetype": "text/x-python",
   "name": "python",
   "nbconvert_exporter": "python",
   "pygments_lexer": "ipython3",
   "version": "3.8.3"
  },
  "latex_envs": {
   "LaTeX_envs_menu_present": true,
   "autoclose": false,
   "autocomplete": true,
   "bibliofile": "biblio.bib",
   "cite_by": "apalike",
   "current_citInitial": 1,
   "eqLabelWithNumbers": true,
   "eqNumInitial": 1,
   "hotkeys": {
    "equation": "Ctrl-E",
    "itemize": "Ctrl-I"
   },
   "labels_anchors": false,
   "latex_user_defs": false,
   "report_style_numbering": false,
   "user_envs_cfg": false
  }
 },
 "nbformat": 4,
 "nbformat_minor": 4
}
