{
 "cells": [
  {
   "cell_type": "markdown",
   "metadata": {},
   "source": [
    "# 1. Mean and variance of the Poisson process\n",
    "\n",
    "The mean and variance are given by \n",
    "\n",
    "\\begin{align*}\n",
    "m(t) &= \\frac{\\partial \\mathcal{P}}{\\partial z}\\Big{|}_{z = 1}, \\\\\n",
    "\\sigma^2(t) &= \\frac{\\partial^2 \\mathcal{P}}{\\partial z^2}\\Big{|}_{z = 1} +  \\frac{\\partial \\mathcal{P}}{\\partial z}\\Big{|}_{z = 1} - \\left(\\frac{\\partial \\mathcal{P}}{\\partial z}\\Big{|}_{z = 1}\\right)^2.\n",
    "\\end{align*}\n",
    "\n",
    "For \n",
    "\n",
    "\\begin{align*}\n",
    "\\mathcal{P}(z,t) = e^{\\lambda (z - 1) t}\n",
    "\\end{align*}\n",
    "\n",
    "we have\n",
    "\n",
    "\\begin{align*}\n",
    "\\frac{\\partial \\mathcal{P}}{\\partial z} = \\lambda t e^{\\lambda(z-1)t} \\\\\n",
    "\\frac{\\partial^2 \\mathcal{P}}{\\partial z^2} = (\\lambda t)^2 e^{\\lambda(z-1)t}\n",
    "\\end{align*}\n",
    "\n",
    "Thus\n",
    "\n",
    "\\begin{align*}\n",
    "m(t) &= \\frac{\\partial \\mathcal{P}}{\\partial z}\\Big{|}_{z = 1} = \\lambda t, \\\\\n",
    "\\sigma^2(t) &= (\\lambda t)^2 + \\lambda t - (\\lambda t)^2 \\\\\n",
    "&= \\lambda t\n",
    "\\end{align*}"
   ]
  },
  {
   "cell_type": "markdown",
   "metadata": {},
   "source": [
    "# 2. Variance of the simple birth process\n",
    "\n",
    "In the notes, we showed that\n",
    "\n",
    "\\begin{align*}\n",
    "m = Ne^{\\lambda t}.\n",
    "\\end{align*}\n",
    "\n",
    "To determine the variance, we multiply the forward Kolmogorov equation by $i^2$ and sum to find\n",
    "\n",
    "\\begin{equation}\\label{eq:q2}\n",
    "\\sum_{i=N}^\\infty i^2 \\frac{dp_i}{dt} = \\sum_{i=N+1}^{\\infty} \\lambda i^2 (i-1) p_{i-1} - \\sum_{i=N}^{\\infty} \\lambda i^3 p_i\n",
    " \\end{equation}\n",
    "\n",
    "We see that \n",
    "\n",
    "\\begin{equation*}\n",
    "\\sum_{i=N}^{\\infty} i^2 \\frac{dp_i}{dt} = \\frac{d}{dt} \\sum_{i=N}^\\infty i^2 p_i \\\\\n",
    "\\sum_{i = N+1}^{\\infty}  \\lambda i^2 (i-1) p_{i-1} = \\sum_{i=N}^\\infty \\lambda (i+1)^2 ip_i\n",
    "\\end{equation*}\n",
    "\n",
    "The RHS of \\eqref{eq:q2} is then\n",
    "\n",
    "\\begin{equation*}\n",
    "\\sum_{i=N}^\\infty \\lambda (i+1)^2 ip_i - \\sum_{i=N}^{\\infty} \\lambda i^3 p_i \\\\\n",
    "= 2 \\lambda \\sum_{i=N}^\\infty i^2 p_i + \\lambda \\sum_{i=N}^\\infty ip_i\n",
    "\\end{equation*}\n",
    "\n",
    "Defining $\\gamma = \\sum_{i=N}^\\infty i^2 p_i$, we have\n",
    "\n",
    "\\begin{equation*}\n",
    "\\frac{d\\gamma}{dt} = 2\\lambda \\gamma + \\lambda m \\\\\n",
    "\\frac{d\\gamma}{dt} - 2\\lambda \\gamma = \\lambda N e^{\\lambda t}\n",
    "\\end{equation*}\n",
    "\n",
    "The general solution is\n",
    "\n",
    "\\begin{equation*}\n",
    "\\gamma = \\gamma_0 e^{2\\lambda t} - Ne^{\\lambda t}\n",
    "\\end{equation*}\n",
    "\n",
    "Since \n",
    "\n",
    "\\begin{align*}\n",
    "\\sigma^2 &= \\sum i^2 p_i - m^2 \\\\\n",
    "&= \\gamma -m^2 \\\\\n",
    "&= \\gamma_0 e^{2\\lambda t} - Ne^{\\lambda t} - N^2e^{2\\lambda t} \\\\\n",
    "&= (\\gamma -N^2)e^{2\\lambda t} - Ne^{\\lambda t}\n",
    "\\end{align*}\n",
    "\n",
    "At $t = 0$ we know $X(0) = N$ and thus $\\sigma^2(0) = 0$.\n",
    "\n",
    "As a result, \n",
    "\n",
    "\\begin{equation*}\n",
    "0 = (\\gamma_0 -N^2)-N \\\\\n",
    "\\gamma_0 = N(N+1) \\\\\n",
    "\\sigma^2(t) = N[e^{2\\lambda t} - e^{\\lambda t}] \\\\\n",
    "= Ne^{\\lambda t}[e^{\\lambda t}-1]\n",
    "\\end{equation*}\n",
    "\n"
   ]
  },
  {
   "cell_type": "markdown",
   "metadata": {},
   "source": [
    "# 3. Simple death process\n",
    "\\begin{enumerate}\n",
    "\n",
    "\\item From the transition probabilities, we see that the non-zero entries of the generator matrix are\n",
    "\n",
    "\\begin{align*}\n",
    "q_{i,i} &= -\\mu i \\\\\n",
    "q_{i-1, i} &= \\mu i\n",
    "\\end{align*}\n",
    "\n",
    "The forward Kolmogorov equation is then \n",
    "\\begin{equation*}\n",
    "\\frac{dp_i}{dt} = -\\mu i p_i + \\mu(i+1)p_{i+1}\n",
    "\\end{equation*}\n",
    "\n",
    "Multiplying by $z^i$ and summing, we have\n",
    "\n",
    "\\begin{equation*}\n",
    "\\frac{d}{dt} \\sum_{i} p_i z^i = -\\mu\\sum_{i} ip_iz^i + \\mu \\sum_{i} (i+1) p_{i+1} z^i\n",
    "\\end{equation*}\n",
    "\n",
    "We can rewrite the sums on the RHS as\n",
    "\n",
    "\\begin{align*}\n",
    "\\sum_{i} i p_i z^i &= z \\sum_{i} i p_i z^{i-1} \\\\\n",
    "  &= z\\frac{\\partial }{\\partial z} (\\sum_{i} p_i z^i )\n",
    "\\end{align*}\n",
    "\n",
    "and\n",
    "\n",
    "\\begin{align*}\n",
    "\\sum_{i}(i+1)p_{i+1}z^i &= \\sum_{i} i p_i z^{i-1} \\\\\n",
    "&= \\frac{\\partial}{\\partial z} \\sum_{i} p_i z^i\n",
    "\\end{align*}\n",
    "\n",
    "Since $\\mathcal{P}(z,t) = \\sum_{i} p_i z^i$ we have that\n",
    "\n",
    "\\begin{equation*}\n",
    "\\frac{\\partial \\mathcal{P}}{\\partial t} = \\mu (1-z) \\frac{\\partial \\mathcal{P}}{\\partial z}\n",
    "\\end{equation*}\n",
    "\n",
    "\\item Introducing $\\tau$ in the usual way, we have\n",
    "\n",
    "\\begin{align*}\n",
    "\\frac{d \\mathcal{P}}{d \\tau} &= 0, \\\\\n",
    "\\frac{dt}{d\\tau} &= 1, \\\\\n",
    "\\frac{dz}{d\\tau} &= \\mu (z-1),\n",
    "\\end{align*}\n",
    "\n",
    "The first two equations give \n",
    "\n",
    "\\begin{equation*}\n",
    "\\mathcal{P}=c_1\\,, t = \\tau + c_2\n",
    "\\end{equation*}\n",
    "\n",
    "The third equation is separable and we see that \n",
    "\n",
    "\\begin{align*}\n",
    "\\int \\frac{dz}{z-1} &= \\int \\mu \\tau \\\\\n",
    "\\log(z-1) &= \\mu \\tau + c \\\\\n",
    "z &= c_3 e^{\\mu \\tau} + 1.\n",
    "\\end{align*}\n",
    "\n",
    "Since the initial data at $\\tau=0$ is given on the $z$ axis which should be parameterised by $s$, we have\n",
    "\n",
    "\\begin{align*}\n",
    "\\mathcal{P}(s,0) &= s^N, \\\\\n",
    "t &= \\tau, \\\\\n",
    "s &= c_3+1\n",
    "\\end{align*}\n",
    "\n",
    "The third equation gives $c_3 = s-1$.\n",
    "\n",
    "Using this in the expression for $z$, we have\n",
    "\n",
    "\\begin{equation*}\n",
    "z = (s-1) e^{\\mu\\tau} +1 .\n",
    "\\end{equation*}\n",
    "\n",
    "Solving for $s$, we see that \n",
    "\n",
    "\\begin{equation*}\n",
    "s = 1+(z-1)e^{-\\mu t}\n",
    "\\end{equation*}\n",
    "\n",
    "Thus, \n",
    "\n",
    "\\begin{equation*}\n",
    "\\mathcal{P}(z,t) = [1+(z-1)e^{-\\mu t}]^N\n",
    "\\end{equation*}\n",
    "\n",
    "\\item From $\\mathcal{P}(z,t)$, we can compute $m$ and $\\sigma^2$.\n",
    "\n",
    "We have \n",
    "\n",
    "\\begin{align*}\n",
    "\\frac{\\partial \\mathcal{P}}{\\partial z} &= N[1+e^{-\\mu t}(z-1)]^{N-1}e^{-\\mu t} \\\\\n",
    "\\frac{\\partial ^2 \\mathcal{P}}{\\partial z^2} &= N(N-1)[1+ e^{-\\mu t}(z-1)]^{N-2} e^{-2\\mu t}\n",
    "\\end{align*}\n",
    "\n",
    "and therefore\n",
    "\n",
    "\\begin{equation*}\n",
    "m(t) = Ne^{-\\mu t}\n",
    "\\end{equation*}\n",
    "\n",
    "and \n",
    "\n",
    "\\begin{align*}\n",
    "\\sigma^2(t) &= N(N-1)e^{-2\\mu t}+Ne^{-\\mu t}-N^2e^{-2\\mu t} \\\\\n",
    "&= Ne^{-\\mu t}(1-e^{-\\mu t}).\n",
    "\\end{align*}\n",
    "\n",
    "\n",
    "\n",
    "\\end{enumerate}"
   ]
  },
  {
   "cell_type": "markdown",
   "metadata": {},
   "source": [
    "# 4. Simple birth and death process with immigration\n",
    "\n",
    "From the transition probabilities, we see that the entries of the generator matrix are \n",
    "\n",
    "\\begin{equation*}\n",
    "q_{i,i} = -\\nu + (\\lambda + \\mu)i \\\\\n",
    "q_{i+1, i}= \\gamma + \\lambda i \\\\\n",
    "q_{i-1,i} = \\mu i\n",
    "\\end{equation*}\n",
    "\n",
    "As a result, the forward Kolmogorov equation is\n",
    "\n",
    "\\begin{equation*}\n",
    "\\frac{dp_i}{dt} = -[\\nu + (\\lambda + \\mu)i]p_i + [\\nu + \\lambda(i-1)]p_{i-1} + \\mu (i+1)p_{i-1}\n",
    "\\end{equation*}\n",
    "\n",
    "We can find the equation for the mean by multiplying the above equation by $i$ and summing such that\n",
    "\n",
    "\\begin{equation*}\n",
    "\\sum_i i\\frac{dp_i}{dt} = -\\sum_i i(\\nu + (\\mu + \\lambda)i)p_i + \\sum_i i (\\nu + \\lambda(i-1))p_{i-1} + \\sum_i \\mu (i+1)p_{i+1}\n",
    "\\end{equation*}\n",
    "\n",
    "We can rewrite two of the sums on the RHS as \n",
    "\n",
    "\\begin{equation*}\n",
    "\\sum_i i (\\nu + \\lambda (i-1))p_{i-1} \\\\\n",
    "= \\sum_i [\\nu + \\lambda i] (i+1) p_i\n",
    " \\end{equation*}\n",
    "\n",
    "and \n",
    "\n",
    "\\begin{equation*}\n",
    "\\sum_i i\\mu(i+1)p_{i+1} = \\sum_i i(i-1)\\mu p_i.\n",
    "\\end{equation*}\n",
    "\n",
    "Using these results and the fact that \n",
    "\n",
    "\\begin{equation*}\n",
    "\\sum_i i \\frac{dp_i}{dt} = \\frac{dm}{dt}\n",
    "\\end{equation*}\n",
    "\n",
    "we have\n",
    "\n",
    "\\begin{equation*}\n",
    "\\frac{dm}{dt} = \\nu + \\lambda m - \\mu m.\n",
    "\\end{equation*}\n",
    "\n",
    "This has the general solution \n",
    "\n",
    "\\begin{equation*}\n",
    "m = ke^{(\\lambda-\\mu)t} + \\frac{\\nu}{\\mu-\\lambda}\n",
    "\\end{equation*}\n",
    "\n",
    "Using the initial condition, $m(0) = N$, we find\n",
    "\n",
    "\\begin{equation*}\n",
    "k = N+\\frac{\\nu}{\\lambda + \\mu}\n",
    "\\end{equation*}\n",
    "\n",
    "and therefore\n",
    "\n",
    "\\begin{equation*}\n",
    "m(t) = Ne^{(\\lambda - \\mu)t} + \\frac{\\nu}{\\lambda - \\mu}[e^{(\\lambda - \\mu)t}-1]\n",
    "\\end{equation*}\n",
    "\n",
    "Based on the rates $\\nu, \\lambda N, -\\mu N$, we have the equation \n",
    "\n",
    "\\begin{equation*}\n",
    "\\frac{dN}{dt} =\\nu + (\\lambda - \\mu) N\n",
    "\\end{equation*}\n",
    "\n",
    "which is precisely the equation for the mean. \n"
   ]
  },
  {
   "cell_type": "markdown",
   "metadata": {},
   "source": [
    "# 5. Burst process\n",
    "\n",
    "\\begin{enumerate}\n",
    "\n",
    "\\item\n",
    "\n",
    "Since the next generation generating function is \n",
    "\\begin{equation*}\n",
    "f(z) = z^{\\beta + 1},\n",
    "\\end{equation*}\n",
    "the backward Kolmogorov differential equation is \n",
    "\\begin{equation*}\n",
    "\\frac{d\\mathcal{P}}{dt}= -\\lambda [\\mathcal{P} - \\mathcal{P}^{\\beta+1}]\\\\\n",
    "= \\lambda\\mathcal{P}[\\mathcal{P}^{\\beta}-1]\n",
    "\\end{equation*}\n",
    "\n",
    "\\item This equation is seperable and accordingly, \n",
    "\\begin{equation*}\n",
    "\\int \\frac{d\\mathcal{P}}{\\mathcal{P}[\\mathcal{P}^{\\beta}-1]} = \\int \\lambda dt \\\\\n",
    "\\frac{1}{\\beta} \\log(1-\\mathcal{P}^{\\beta})-\\log \\mathcal{P} = \\lambda t + c_0 \\\\\n",
    "\\frac{1-\\mathcal{P}^{\\beta}}{\\mathcal{P}^{\\beta}} = ke^{\\beta \\lambda t}\n",
    "\\end{equation*}\n",
    "Since at $t=0$, $\\mathcal{P} = z$, \n",
    "\\begin{equation*}\n",
    "\\frac{1-z^{\\beta}}{z^{\\beta}} = k\n",
    "\\end{equation*}\n",
    "And therefore\n",
    "\\begin{equation*}\n",
    "\\frac{1-\\mathcal{P}^{\\beta}}{\\mathcal{P}^{\\beta}} = \\frac{1-z^\\beta}{z^\\beta}e^{\\beta \\lambda t}.\n",
    "\\end{equation*}\n",
    "Solving for $\\mathcal{P}$, we find \n",
    "\\begin{equation*}\n",
    "\\mathcal{P}(z,t) = [1+e^{\\beta \\lambda t}(z^{-\\beta}-1)]^{\\frac{-1}{\\beta}}\n",
    "\\end{equation*}\n",
    "\n",
    "\\item\n",
    "\n",
    "The mean is given by \n",
    "\\begin{align*}\n",
    "m(t) &= \\frac{\\partial \\mathcal{P}}{\\partial z}\\Big{|}_{z = 1}\n",
    "\\end{align*}\n",
    "\n",
    "As\n",
    "\\begin{equation*}\n",
    "\\frac{\\partial \\mathcal{P}}{\\partial z} = \\frac{e^{\\beta \\lambda t}z^{-(\\beta -1)}}{[1+ e^{\\beta \\lambda t}(z^{-\\beta} -1)]^{1+\\frac{1}{\\beta}}}\n",
    "\\end{equation*}\n",
    "we have\n",
    "\\begin{equation*}\n",
    "m(t) = e^{\\beta \\lambda t}\n",
    "\\end{equation*}\n",
    "\n",
    "\n",
    "\\end{enumerate}"
   ]
  },
  {
   "cell_type": "markdown",
   "metadata": {},
   "source": [
    "# 6. Bivariate birth and death process\n",
    "\n",
    "The forward Kolmogorov equation for this process is given in the notes and is \n",
    "\n",
    "\\begin{align*}\n",
    "\\frac{d p_{(m,n)}}{d t} &= - p_{(m,n)}(t) \\left((\\lambda_1 + \\mu_1)m + (\\lambda_2 + \\mu_2)n\\right) \\\\\n",
    "&+ \\lambda_1(m-1)p_{(m-1,n)}(t) + \\lambda_2(n-1)p_{(m,n-1)}(t)\\\\\n",
    "&+ \\mu_1(m+1)p_{(m+1,n)}(t) + \\mu_2(n+1)p_{(m,n+1)}(t).\n",
    "\\end{align*}\n",
    "\n",
    "Let's first find \n",
    "\\begin{align*}\n",
    "\\mu_X &= \\sum_{m = 0}^{\\infty}\\sum_{n = 0}^{\\infty}m p_{(m,n)}(t)\n",
    "\\end{align*}\n",
    "\n",
    "To do so, we multiply the FKE by $m$ and sum over $(m,n)$ to find\n",
    "\\begin{align}\n",
    "\\sum_{(m,n)} m \\frac{d p_{(m,n)}}{dt} &= \\frac{d \\mu_X}{dt} \\nonumber \\\\\n",
    "&= - \\sum_{(m,n)}p_{(m,n)}(t) m\\left((\\lambda_1 + \\mu_1)m + (\\lambda_2 + \\mu_2)n\\right) \\nonumber \\\\\n",
    "&+ \\sum_{(m,n)}\\lambda_1 m (m-1)p_{(m-1,n)}(t) + \\sum_{(m,n)}\\lambda_2 m(n-1)p_{(m,n-1)}(t) \\nonumber \\\\\n",
    "&+ \\sum_{(m,n)}\\mu_1m(m+1)p_{(m+1,n)}(t) + \\sum_{(m,n)}\\mu_2m(n+1)p_{(m,n+1)}(t) \\label{eq:q6}\n",
    "\\end{align}\n",
    "\n",
    "We can rewrite the following sums as \n",
    "\\begin{align*}\n",
    "\\sum_{(m,n)}\\lambda_1m(m-1)p_{(m-1,n)}(t) &= \\sum_{(m,n)}\\lambda_1(m+1)mp_{(m,n)}(t) \\\\\n",
    "\\sum_{(m,n)}\\lambda_2m(n-1)p_{(m,n-1)}(t) &= \\sum_{(m,n)}\\lambda_2 mnp_{(m,n)}(t) \\\\\n",
    "\\sum_{(m,n)}\\mu_1m(m+1)p_{(m+1,n)}(t) &= \\sum_{(m,n)}\\mu_1(m-1)mp_{(m,n)}(t) \\\\\n",
    "\\sum_{(m,n)}\\mu_2m(n+1)p_{(m,n+1)}(t) &= \\sum_{(m,n)}\\mu_2mnp_{(m,n)}(t).\n",
    "\\end{align*}\n",
    "\n",
    "Using these results in \\eqref{eq:q6} above, we have\n",
    "\\begin{equation*}\n",
    "\\frac{d \\mu_X}{dt} = \\lambda_1 \\sum_{(m,n)} mp_{(m,n)} - \\mu_1\\sum_{(m,n)} mp_{(m,n)}\n",
    "\\end{equation*}\n",
    "and therefore,\n",
    "\n",
    "\\begin{equation*}\n",
    "\\frac{d \\mu_X}{dt} = (\\lambda_1-\\mu_1)\\mu_X.\n",
    "\\end{equation*}\n",
    "\n",
    "By similar arguments, we also have \n",
    "\\begin{equation*}\n",
    "\\frac{d \\mu_Y}{dt} = (\\lambda_2-\\mu_2)\\mu_Y.\n",
    "\\end{equation*}"
   ]
  },
  {
   "cell_type": "markdown",
   "metadata": {},
   "source": [
    "# 7. Noise propagation in a gene expression\n",
    "\\begin{enumerate}\n",
    "\n",
    "\\item The law of mas action gives the deterministic equations\n",
    "\\begin{equation*}\n",
    "\\frac{dm}{dt} = \\underbrace{k_1}_{\\lambda_1} - \\underbrace{k_m m}_{\\mu_1} \\\\\n",
    "\\frac{dp}{dt} = \\underbrace{k_2 m}_{\\lambda_2} - \\underbrace{k_p p}_{\\mu_2}\n",
    "\\end{equation*}\n",
    "\n",
    "This is a bivariate birth and death process with birth rates $\\lambda_1 = \\tilde{k}_1$ and $\\lambda_2$, and death rates $\\mu_1$ and $\\mu_2$, as indicated in the equation above.  Accordingly, the transition probabilities correspond to those in question 6 and with the forward Kolmogorov equation given in the notes.  Then, multiplying the forward Kolmogorov differential equation by $m$ and summing, we obtain\n",
    "\n",
    "\\begin{align*}\n",
    "\\frac{d\\mu_m}{dt} = &-\\sum_{(m,n)}m p_{(m,n)}[\\tilde{k}_1 + k_mm + k_2m + k_p n] \\\\\n",
    "&+ \\sum_{(m,n)}m \\tilde{k}_1 p_{(m-1,n)} \\\\\n",
    "&+ \\sum_{(m,n)}m (m+1)k_m p_{(m+1,n)} \\\\\n",
    "&+ \\sum_{(m,n)}m^2 k_2 p_{(m,n-1)} \\\\\n",
    "&+ \\sum_{(m,n)}m(n+1) k_p p_{(m,n+1)} \n",
    "\\end{align*}\n",
    "\n",
    "Rearranging in a similar way to the Q6 solutions, we find\n",
    "\n",
    "\\begin{equation*}\n",
    "\\frac{d\\mu_m}{dt} = \\tilde{k}_1\\sum_{(m,n)}p_{(m,n)} - k_m \\sum_{(m,n)} mp_{(m,n)} \\\\\n",
    "= \\tilde{k}_1 -k_m \\mu_m\n",
    "\\end{equation*}\n",
    "\n",
    "We now multiply the forward Kolmogorov equation by $n$, sum over $(m,n)$, and rearrange the sums.  In doing so, we obtain\n",
    "\n",
    "\\begin{equation*}\n",
    "\\frac{d\\mu_p}{dt} = k_2\\mu_m -k_p\\mu_p\n",
    "\\end{equation*}\n",
    "\n",
    "\\item For the variance $\\sigma^2_m$, we multiply the FK equation by $m^2$ and sum over $(m,n)$.  We then rearrange and combine the terms to give\n",
    "\n",
    "\\begin{equation*}\n",
    "\\frac{d}{dt} \\sum_{(m,n)}m^2 p_{(m,n)} = 2\\tilde{k}_1 \\mu_m + \\tilde{k}_1-k_m \\sum_{(m,n)}m^2 p_{(m,n)} \\\\\n",
    "\\end{equation*}\n",
    "\n",
    "Thus for $\\sigma^2_m$, we have that\n",
    "\n",
    "\\begin{equation*}\n",
    "\\frac{d\\sigma^2}{dt} = \\frac{d}{dt}(\\sum_{(m,n)} m^2 p_{(m,n)}) -2\\mu_m \\frac{d\\mu_m}{dt} \\\\\n",
    "\\frac{d\\sigma^2_m}{dt} = \\tilde{k}_1 - 2k_m \\sigma_m^2 + k_m \\mu_m \n",
    "\\end{equation*}\n",
    "\n",
    "Similarly, for $\\sigma^2_p$, we consider $\\frac{d}{dt} \\sum_{(m,n)}n^2 p_{(m,n)}$ and ultimately find that\n",
    "\n",
    "\\begin{equation*}\n",
    "\\frac{d\\sigma_p^2}{dt} = \\frac{d}{dt}(\\sum_{(m,n)}n^2p_{(m,n)}) - 2\\mu_p \\frac{d\\mu_p}{dt}\\\\\n",
    "= k_2 \\mu_m + k_p\\mu_p - 2k_p\\sigma^2_p + 2k_2\\sigma_{mp}\n",
    "\\end{equation*}\n",
    "\n",
    "where\n",
    "\n",
    "\\begin{equation*}\n",
    "\\sigma_{mp} = \\sum_{(m,n)}mnp_{(m,n)} - \\mu_m \\mu_p.\n",
    "\\end{equation*}\n",
    "\n",
    "We see then that we will also need to find the equation for $\\sigma_{mp}$.  Thus, we consider $\\frac{d}{dt} \\sum_{(m,n)}mn p_{(m,n)}$.  Following the usual procedure, we find \n",
    "\n",
    "\\begin{equation*}\n",
    "\\frac{d}{dt}\\sigma_{mp} = \\frac{d}{dt}(\\sum_{(m,n)}mnp_{(m,n)}) - \\frac{d\\mu_p}{dt}\\mu_m - \\mu_p \\frac{d\\mu_m}{dt}\\\\\n",
    "= - k_m\\sigma_{mp}+k_2\\sigma^2_m - k_p \\sigma_{mp}\n",
    "\\end{equation*}\n",
    "\n",
    "At steady-state where the time derivatives are zero, \n",
    "\\begin{equation*}\n",
    "\\tilde{k}_1 =\\mu_m, \\\\\n",
    "\\mu_m=\\frac{k_p \\mu_p}{k_2}, \\\\\n",
    "\\sigma_m^2 = \\mu_m, \\\\\n",
    "\\sigma_{mp} = \\frac{k_2}{k_m + k_p} \\sigma^2_m, \\\\\n",
    "\\sigma_p^2 = \\mu_p + \\frac{k_2}{k_p} \\sigma_{mp}.\n",
    "\\end{equation*}\n",
    "\n",
    "Based on these equations, we see that\n",
    "\\begin{equation*}\n",
    "\\frac{\\sigma_m^2}{\\mu_m^2} = \\frac{1}{\\mu_m} \\\\ \n",
    "\\frac{\\sigma_p^2}{\\mu_p^2} = \\frac{1}{\\mu_p} + \\frac{k_2}{k_p} \\frac{k_2}{k_m+k_p} \\frac{\\sigma_m^2}{\\mu^2_p} \\\\\n",
    "= \\frac{1}{\\mu_p} + \\frac{\\gamma}{1+\\gamma} \\frac{\\sigma_m^2}{\\mu_m^2}\n",
    "\\end{equation*}\n",
    "where $\\gamma = \\frac{k_p}{k_m}$.\n",
    "\n",
    "\\item If $\\gamma \\gg 1$ i.e. the protein decays much faster than the mRNA, then the variability in the protein concentration will be inherited from the mRNA values.\n",
    "\n",
    "If $\\gamma \\ll 1$, then we have $\\frac{\\sigma_p^2}{\\mu_p^2} \\approx \\frac{1}{\\mu_p}$ which is independent of mRNA variability. \n",
    "\n",
    "\n",
    "\\end{enumerate}"
   ]
  }
 ],
 "metadata": {
  "kernelspec": {
   "display_name": "Python 3",
   "language": "python",
   "name": "python3"
  },
  "language_info": {
   "codemirror_mode": {
    "name": "ipython",
    "version": 3
   },
   "file_extension": ".py",
   "mimetype": "text/x-python",
   "name": "python",
   "nbconvert_exporter": "python",
   "pygments_lexer": "ipython3",
   "version": "3.8.3"
  },
  "latex_envs": {
   "LaTeX_envs_menu_present": true,
   "autoclose": false,
   "autocomplete": true,
   "bibliofile": "biblio.bib",
   "cite_by": "apalike",
   "current_citInitial": 1,
   "eqLabelWithNumbers": true,
   "eqNumInitial": 1,
   "hotkeys": {
    "equation": "Ctrl-E",
    "itemize": "Ctrl-I"
   },
   "labels_anchors": false,
   "latex_user_defs": false,
   "report_style_numbering": false,
   "user_envs_cfg": false
  }
 },
 "nbformat": 4,
 "nbformat_minor": 4
}
